lakefile.lean
@@ -1,0 +1,12 @@
+import Lake
+open Lake DSL
+
+package poincare_new_derivation where
+  leanOptions := #[⟨`pp.unicode.fun, true⟩]
+
+require mathlib from git
+  "https://github.com/leanprover-community/mathlib4"
+
+@[default_target]
+lean_lib Poincare where
+  srcDir := "lean"
